theories/AlmostStlc/TypesEquiv.v
@@ -3,9 +3,11 @@ Require Export SyntaxSeq.
 Require Export SmallStepSeq.
 Require Export DenotationFacts.
 Require Export DenotationSeq.
+Require Export Eqit.
 Require Export Rutt.
 Require Export RuttFacts.
 Require Import ITree.Basics.HeterogeneousRelations.
+Require Export InterpMTreeFacts.
 Import List.ListNotations.
 Open Scope list_scope.
 From Equations Require Import Equations Signature.
@@ -18,38 +20,6 @@ Inductive list_rel {A} (R : Rel A A): Rel (list A) (list A) :=
   | list_rel_nil : list_rel R nil nil
   | list_rel_cons a b l1 l2 : R a b ->list_rel R l1 l2 -> list_rel R (cons a l1) (cons a l2).
 
-Section types_equiv.
-
-(*
-
-Inductive types_equiv : forall t : type, Rel (denote_type t) (denote_type t) := 
-  | types_equiv_Nat n : types_equiv Nat n n
-  | types_equiv_Pair t1 t2 p1 p2 : prod_rel (types_equiv t1) (types_equiv t2) p1 p2 ->
-                                   types_equiv (Pair t1 t2) p1 p2
-  | types_equiv_List t l1 l2 : list_rel (types_equiv t) l1 l2 ->
-                               types_equiv (List t) l1 l2
-  | types_equiv_Arrow t1 MR t2 f g : 
-    (forall x y, types_equiv t1 x y -> rutt hole hole (types_equiv t2) (f x) (g x) ) ->
-    types_equiv (Arrow t1 MR t2) f g
-.
-the arrow type requires non strict positive application, needs to be a fixpoint
-
-
-*)
-
-(* seems to not be recognizing  that this is well founded, probably a dependent 
-   pattern matching problem, first thing to try might be to do this in equations
-   after that maybe consider some gas-like solution
-
-   this might take much of tomorrow, I am concerned about the march deadline,
-   but if we miss it thats not really a problem talk about the next deadline with steve next week
-
-  *)
-(* maybe also create a generalized version of this so that we can get some more 
-   general equational theory working 
-   maybe also a relation for any mtree, built on top of rutt and do some of the 
-   theory at that level
-*)
 Equations types_equiv (t : type) : Rel (denote_type t) (denote_type t) := {
     types_equiv Nat := eq;
     types_equiv (Pair t1 t2) := prod_rel (types_equiv t1) (types_equiv t2);
@@ -97,7 +67,342 @@ Definition comp_equiv {t Γ MR} :=
     fun c1 c2 => forall hyps1 hyps2, ctx_equiv Γ hyps1 hyps2 ->
               rutt (mfix_pre_equiv MR) (mfix_post_equiv MR) (types_equiv t) (c1 hyps1) (c2 hyps2).
 
+Lemma mfix_pre_call_mrec:
+    forall (t1 t2 : vtype) (MR : mfix_ctx) (R : call_frame) (xR : var R MR) 
+           (x : var (t1, t2) R) (r1 r2 : denote_type t1) (c1 : denote_mrec_ctx (denote_mfix_ctx MR))
+           (f1 : encodes c1 -> denote_type t2) (c2 : denote_mrec_ctx (denote_mfix_ctx MR))
+           (f2 : encodes c2 -> denote_type t2),
+      types_equiv t1 r1 r2 ->
+      call_mrec x xR r1 = c1 && f1 -> call_mrec x xR r2 = c2 && f2 -> mfix_pre_equiv MR c1 c2.
+Proof.
+  intros t1 t2 MR R xR x r1 r2 c1 f1 c2 f2.
+  dependent induction xR.
+  - simp call_mrec. intros. rewrite mfix_pre_equiv_equation_2.
+    destruct (call_mrec_call_frame x r1) as [d1 g1] eqn : Heq1.
+    destruct (call_mrec_call_frame x r2) as [d2 g2] eqn : Heq2.
+    inversion H1. subst. inversion H0. subst. constructor.
+    rename a into R. revert Heq1 Heq2 H. clear H0 H1.
+    dependent induction x.
+    + simp call_mrec_call_frame. intros.
+      inversion Heq1. inversion Heq2. subst. constructor. auto.
+    + destruct b as [t3 t4]. simp call_mrec_call_frame.
+      rewrite call_frame_pre_equiv_equation_2. intros.
+      destruct (call_mrec_call_frame x r1) as [d3 g3] eqn : Heq3.
+      destruct (call_mrec_call_frame x r2) as [d4 g4] eqn : Heq4.
+      inversion Heq1. inversion Heq2. subst. constructor.
+      eapply IHx; eauto.
+  - simp call_mrec. intros. rewrite mfix_pre_equiv_equation_2.
+    destruct (call_mrec x xR r1) as [d1 g1] eqn : Heq1.
+    destruct (call_mrec x xR r2) as [d2 g2] eqn : Heq2.
+    specialize (IHxR x r1 r2 d1 g1 d2 g2 H Heq1 Heq2).
+    inversion H0. inversion H1. constructor. auto.
+Qed.
 
+Lemma mfix_post_equiv_types_equiv_aux:
+  forall (t1 t2 : vtype) (MR : mfix_ctx) (R : call_frame) (xR : var R MR) 
+    (x : var (t1, t2) R) (r1 r2 : denote_type t1) (c1 : denote_mrec_ctx (denote_mfix_ctx MR))
+    (f1 : encodes c1 -> denote_type t2),
+    call_mrec x xR r1 = c1 && f1 ->
+    forall (c2 : denote_mrec_ctx (denote_mfix_ctx MR)) (f2 : encodes c2 -> denote_type t2),
+      call_mrec x xR r2 = c2 && f2 ->
+      encodes c1 = denote_type t2 ->
+      encodes c2 = denote_type t2 ->
+      f1 ~= @id (denote_type t2) ->
+      f2 ~= @id (denote_type t2) ->
+      forall (a : encodes c1) (b : encodes c2),
+        mfix_post_equiv MR c1 c2 a b -> types_equiv t2 (f1 a) (f2 b).
+Proof.
+  intros t1 t2 MR R xR x r1 r2 c1 f1 Heq1 c2 f2 Heq2 Henc1 Henc2 Hcont1 Hcont2 a b Hab.
+  dependent induction xR.
+  - rewrite mfix_post_equiv_equation_2 in Hab.
+    simp call_mrec in Heq1, Heq2.
+    destruct (call_mrec_call_frame x r1) as [d1 g1] eqn : Heq3.
+    destruct (call_mrec_call_frame x r2) as [d2 g2] eqn : Heq4.
+    inversion Heq1. inversion Heq2. subst.
+    apply Eqdep.EqdepTheory.inj_pair2 in Heq1, Heq2. subst.
+    dependent destruction Hab.
+    dependent induction x.
+    + rewrite call_frame_post_equiv_equation_2 in H3.
+      simp call_mrec_call_frame in Heq3, Heq4.
+      inversion Heq3. inversion Heq4. subst.
+      dependent destruction H3. cbn in f1, f2.
+      unfold inout_encoded in f1, f2. apply JMeq_eq in Hcont1, Hcont2.
+      subst. auto.
+    + destruct b. rewrite call_frame_post_equiv_equation_2 in H3.
+      simp call_mrec_call_frame in Heq3, Heq4.
+      inversion Heq3. inversion Heq4. subst.
+      destruct (call_mrec_call_frame x r1) as [d1' g1'] eqn : Heq5.
+      destruct (call_mrec_call_frame x r2) as [d2' g2'] eqn : Heq6.
+      inversion H0. inversion H1. subst.
+      dependent destruction H3.
+      apply Eqdep.EqdepTheory.inj_pair2 in H0, H1. subst.
+      eapply IHx; eauto.
+  - rewrite mfix_post_equiv_equation_2 in Hab.
+    simp call_mrec in Heq1, Heq2.
+    destruct (call_mrec x xR r1) as [d1 g1] eqn : Heq3.
+    destruct (call_mrec x xR r2) as [d2 g2] eqn : Heq4.
+    inversion Heq1. inversion Heq2.
+    subst. dependent destruction Hab.
+    apply Eqdep.EqdepTheory.inj_pair2 in Heq1, Heq2.
+    subst.
+    eapply IHxR in H3; eauto.
+Qed.
+
+Lemma mfix_post_equiv_types_equiv:
+  forall (t1 t2 : vtype) (MR : mfix_ctx) (R : call_frame) (xR : var R MR) 
+    (x : var (t1, t2) R) (r1 r2 : denote_type t1) (c1 : denote_mrec_ctx (denote_mfix_ctx MR))
+    (f1 : encodes c1 -> denote_type t2),
+    call_mrec x xR r1 = c1 && f1 ->
+    forall (c2 : denote_mrec_ctx (denote_mfix_ctx MR)) (f2 : encodes c2 -> denote_type t2),
+      call_mrec x xR r2 = c2 && f2 ->
+      forall (a : encodes c1) (b : encodes c2),
+        mfix_post_equiv MR c1 c2 a b -> types_equiv t2 (f1 a) (f2 b).
+Proof.
+  intros. eapply mfix_post_equiv_types_equiv_aux; eauto.
+  - specialize (call_mrec_encodes _ _ _ _ x xR r1) as Henc1. rewrite <- Henc1.
+    rewrite H. auto.
+  - specialize (call_mrec_encodes _ _ _ _ x xR r2) as Henc2. rewrite <- Henc2.
+    rewrite H0. auto.
+  - specialize (call_mrec_cont _ _ _ _ x xR r1) as Hcont1. rewrite H in Hcont1.
+    auto.
+  - specialize (call_mrec_cont _ _ _ _ x xR r2) as Hcont2. rewrite H0 in Hcont2.
+    auto.
+Qed.
+
+Lemma comp_equiv_call (t1 t2 : type) Γ MR R (xR : var R MR) (x : var (t1,t2) R) 
+      (v1 v2 : value t1 Γ): 
+  comp_equiv (MR := MR) (denote_value v1) (denote_value v2) ->
+  comp_equiv (denote_comp (comp_call xR x v1)) (denote_comp (comp_call xR x v2)).
+Proof.
+  intros. red. intros.
+  simp denote_comp.
+  eapply rutt_bind; eauto.
+  intros.
+  unfold call_term.
+  destruct (call_mrec x xR r1) as [c1 f1] eqn : Heq1.
+  destruct (call_mrec x xR r2) as [c2 f2] eqn : Heq2. 
+  setoid_rewrite bind_trigger. apply rutt_Vis.
+  eapply mfix_pre_call_mrec; eauto.
+  intros. apply rutt_Ret. eapply mfix_post_equiv_types_equiv; eauto.
+Qed.
+
+
+
+(*
+now show that for any d1 : denote MR, exists R t1 t2 xR x,
+  d1 = projT1 (call_mrec x xR v1)
+
+  then do these lemmas for insert rel
+
+Lemma mfix_pre_equiv_position_inv (MR : mfix_ctx) 
+      (d1 d2 : denote_mrec_ctx (denote_mfix_ctx MR)) :
+  mfix_pre_equiv MR d1 d2 ->
+  exists R (t1 t2 : type) (xR : var R MR) (x : var (t1,t2)),
+  d1 = projT1 (call_mrec x xR v1) ->
+  d2 = projT1 (call_mrec x xR v2) ->
+  types_equiv t1 v1 v2 ->
+  m.
+Proof.
+() *)
+      (*
+InsertPreRel :
+forall {MR1 MR2 : mrec_ctx} {In1 In2 : Type} {Out1 : EncodedType In1} {Out2 : EncodedType In2} (x : var (In1 && Out1) MR1)
+  (y : var (In2 && Out2) MR2),
+Rel In1 In2 -> Rel (denote_remainder MR1 x) (denote_remainder MR2 y) -> Rel (denote_mrec_ctx MR1) (denote_mrec_ctx MR2)
+
+mfix_pre_equiv
+     : forall MR : mfix_ctx, Rel (denote_mrec_ctx (denote_mfix_ctx MR)) (denote_mrec_ctx (denote_mfix_ctx MR))
+
+call_frame_pre_equiv
+     : forall cf : call_frame, Rel (denote_call_frame cf) (denote_call_frame cf)
+*)
+(*
+The term "mfix_pre_equiv (remove R MR xR)" has type
+ "Rel (denote_mrec_ctx (denote_mfix_ctx (remove R MR xR))) (denote_mrec_ctx (denote_mfix_ctx (remove R MR xR)))"
+while it is expected to have type
+ "Rel (denote_remainder (denote_mfix_ctx MR) (denote_var xR)) (denote_remainder (denote_mfix_ctx MR) (denote_var xR))"
+(cannot unify "denote_remainder (denote_mfix_ctx MR) (denote_var xR)" and "denote_mrec_ctx (denote_mfix_ctx (remove R MR xR))"
+
+need some kind of lift thing to commute
+
+*)
+
+
+(*
+Lemma insert_pre_rel_mfix_pre_equiv_aux1:
+  forall (a b : call_frame) (l : mfix_ctx) (xR : var a l)
+    (d : denote_mrec_ctx (denote_mfix_ctx' (List.map (List.map (fun '(t1, t2) => denote_type t1 && inout_encoded (denote_type t1) (denote_type t2))) l)))
+    (d0 : denote_mrec_ctx (denote_mfix_ctx' (List.map (List.map (fun '(t1, t2) => denote_type t1 && inout_encoded (denote_type t1) (denote_type t2))) l)))
+                 (a1 a2 : denote_call_frame a),
+    inl a2 = projT1 (bring_to_front (denote_mfix_ctx (b :: l)) (VarS (denote_var xR)) (inr d0)) ->
+    inl a1 = projT1 (bring_to_front (denote_mfix_ctx (b :: l)) (VarS (denote_var xR)) (inr d)) ->
+    call_frame_pre_equiv a a1 a2 ->
+    sum_rel (call_frame_pre_equiv a) (commute_remove_rel (mfix_pre_equiv (remove a l xR))) (projT1 (bring_to_front (denote_mfix_ctx l) (denote_var xR) d))
+            (projT1 (bring_to_front (denote_mfix_ctx l) (denote_var xR) d0)).
+Abort.
+
+Lemma insert_pre_rel_equiv_comp_equiv_aux2:
+  forall (a b : call_frame) (l : mfix_ctx) (xR : var a l) (x0 y : denote_mrec_ctx (denote_mfix_ctx (b :: l)))
+    (b1 b2 : denote_remainder (denote_mfix_ctx (b :: l)) (denote_var (VarS xR))),
+    commute_remove_rel (mfix_pre_equiv (remove a (b :: l) (VarS xR))) b1 b2 ->
+    (forall x y : denote_mrec_ctx (denote_mfix_ctx l),
+         InsertPreRel (denote_var xR) (denote_var xR) (call_frame_pre_equiv a) (commute_remove_rel (mfix_pre_equiv (remove a l xR))) x
+           y <-> mfix_pre_equiv l x y) ->
+    inr b1 = projT1 (bring_to_front (denote_mfix_ctx (b :: l)) (VarS (denote_var xR)) x0) ->
+    inr b2 = projT1 (bring_to_front (denote_mfix_ctx (b :: l)) (VarS (denote_var xR)) y) -> mfix_pre_equiv (b :: l) x0 y.
+Proof.
+  intros a b l xR x0 y b1 b2.
+  intros Hb12 IH Hb1 Hb2. red in Hb12. 
+  Transparent remove_denote. Transparent remove.
+  destruct (bring_to_front (denote_mfix_ctx (b :: l)) (VarS (denote_var xR)) x0) eqn : Heq1.
+  simpl in Hb1. subst.
+  destruct (bring_to_front (denote_mfix_ctx (b :: l)) (VarS (denote_var xR)) y) eqn : Heq2.
+  simpl in Hb2. subst.
+  simpl remove in Hb12. simpl in Hb12. 
+  dependent destruction Hb12.
+  - destruct b1; destruct b2.
+    * injection x1; injection x; intros; subst. clear x x1.
+      fold call_frame_pre_equiv in H.
+      destruct x0; destruct y.
+      -- constructor. fold call_frame_pre_equiv.
+         setoid_rewrite bring_to_front_equation_4 in Heq1.
+         setoid_rewrite bring_to_front_equation_4 in Heq2.
+         injection Heq1. intros. subst.
+         injection Heq2. intros. subst. auto.
+      -- setoid_rewrite bring_to_front_equation_5 in Heq2.
+         match goal with H : (let (x,f) := ?t in _ ) = _ |- _ =>
+                           destruct t as [ [? | ?] ? ]; discriminate end.
+      -- setoid_rewrite bring_to_front_equation_5 in Heq1.
+         match goal with H : (let (x,f) := ?t in _ ) = _ |- _ =>
+                           destruct t as [ [? | ?] ? ]; discriminate end.
+      -- constructor.
+         setoid_rewrite bring_to_front_equation_5 in Heq1.
+         match goal with H : (let (x,f) := ?t in _ ) = _ |- _ =>
+                           destruct t as [ [? | ?] ? ]; discriminate end.
+    * destruct (remove_denote xR d0); discriminate.
+    * destruct (remove_denote xR d); discriminate.
+    * destruct (remove_denote xR d); discriminate.
+  - destruct b1 eqn : Hb1'; try discriminate. destruct b2 eqn : Hb2'; try discriminate.
+    (**)
+    destruct x0; destruct y.
+    + constructor. fold call_frame_pre_equiv.
+      setoid_rewrite bring_to_front_equation_4 in Heq1. discriminate.
+    + setoid_rewrite bring_to_front_equation_4 in Heq1. discriminate.
+    + setoid_rewrite bring_to_front_equation_4 in Heq2. discriminate.
+    + setoid_rewrite bring_to_front_equation_5 in Heq1.
+      match goal with H : (let (x,f) := ?t in _ ) = _ |- _ =>
+                           destruct t as [ [? | ?] ? ] eqn : Heq3; try discriminate end.
+      injection Heq1. intros. subst. clear Heq1.
+      setoid_rewrite bring_to_front_equation_5 in Heq2.
+      match goal with H : (let (x,f) := ?t in _ ) = _ |- _ =>
+                           destruct t as [ [? | ?] ? ] eqn : Heq4; try discriminate end.
+      injection Heq2. intros. subst. clear Heq2.
+      constructor.
+      destruct (remove_denote xR d0) as [d0' ?] eqn : Heq5.
+      destruct (remove_denote xR d) as [d' ?] eqn : Heq6.
+      injection x. injection x1. intros. subst. clear x x1 IH.
+      (* possible that this case requires induction on xR 
+         
+
+       *)
+Abort. *)
+(* how would insert pre rel work with mfix pre rel 
+
+maybe consider using the position relation,
+if related, x and y must have the same position
+
+if they both have a position, then this relation reduces down 
+to the types equiv stuff, in any case call it for now
+
+*)
+
+(*
+       split.
+    + simpl denote_var. unfold InsertPreRel. 
+      intros. rewrite mfix_pre_equiv_equation_2.
+      simpl denote_mfix_ctx in H.
+      dependent destruction H.
+      * simp bring_to_front in x1.
+        simpl in x0, y.
+        destruct x0; destruct y; 
+        try setoid_rewrite bring_to_front_equation_2 in x1;
+        try setoid_rewrite bring_to_front_equation_2 in x;
+          try discriminate.
+        cbn in x, x1. injection x. injection x1. intros. subst.
+        constructor. auto.
+      * destruct x0; destruct y; 
+          try setoid_rewrite bring_to_front_equation_3 in x1;
+          try setoid_rewrite bring_to_front_equation_3 in x;
+          try discriminate.
+        injection x1. injection x. intros; subst.
+        constructor.
+        red in H.
+        assert (remove a (a :: l) VarZ  = l).
+        simp remove. auto.
+        setoid_rewrite remove_denote_equation_1 in H.
+        cbn in H.
+        clear - H. Transparent remove. cbn in H.
+        Opaque remove. auto.
+   + intros. rewrite mfix_pre_equiv_equation_2 in H.
+     red. dependent destruction H.
+     * constructor. auto.
+     * constructor. red.
+       setoid_rewrite remove_denote_equation_1.
+       Transparent remove. cbn. Opaque remove. auto.          
+  - split; intros.
+    + red in H. dependent destruction H.
+      * Transparent denote_var. simpl denote_var in x1, x.
+        destruct x0; destruct y;
+        try setoid_rewrite bring_to_front_equation_2 in x1;
+        try setoid_rewrite bring_to_front_equation_2 in x;
+          try discriminate.
+        constructor. apply IHxR. red.
+        eapply insert_pre_rel_mfix_pre_equiv_aux1; eauto.
+      * simpl denote_var in x, x1, H.
+        revert H x1 x.
+        red in H. admit.
+    + red in H. dependent destruction H. 
+      * do 2 constructor; auto.
+      * simpl denote_var. red. 
+        eapply IHxR in H. red in H.
+        dependent destruction H.
+        -- destruct 
+            ((bring_to_front (denote_mfix_ctx l) (denote_var xR) b1))
+            eqn : Heq1; cbn in x0; subst; try discriminate.
+          unfold denote_mfix_ctx. simpl.
+            rewrite bring_to_front_equation_5.
+            setoid_rewrite Heq1.
+            simpl.
+             destruct 
+            ((bring_to_front (denote_mfix_ctx l) (denote_var xR) b2))
+            eqn : Heq2; cbn in x; subst; try discriminate.
+          unfold denote_mfix_ctx. simpl.
+            rewrite bring_to_front_equation_5.
+            setoid_rewrite Heq2. constructor.
+            auto.
+       -- destruct 
+            ((bring_to_front (denote_mfix_ctx l) (denote_var xR) b1))
+            eqn : Heq1; cbn in x0; subst; try discriminate.
+          unfold denote_mfix_ctx. simpl.
+            rewrite bring_to_front_equation_5.
+            setoid_rewrite Heq1.
+            simpl.
+             destruct 
+            ((bring_to_front (denote_mfix_ctx l) (denote_var xR) b2))
+            eqn : Heq2; cbn in x; subst; try discriminate.
+          unfold denote_mfix_ctx. simpl.
+            rewrite bring_to_front_equation_5.
+            setoid_rewrite Heq2.
+            constructor.
+            clear - H. red. Transparent remove_denote.
+            red in H.
+            simpl remove_denote.
+            Transparent remove. simpl remove. simpl.
+            destruct (remove_denote xR b0);
+            destruct (remove_denote xR b3).
+            constructor. auto.
+Admitted. *)
+(* lets put this part aside for a bit and focus on another part *)
 (*
 Should be a PER 
 
@@ -117,5 +422,7 @@ other things might actually include some bugs
 
 on monday work on this but also dedicate some time to the proposal intro
 
+
+also maybe go back to the comp_map proof and see what kind of reasoning principles are needed
 
 *)
