theories/AlmostStlc/TypesEquivPrePostRel.v
@@ -1,0 +1,667 @@
+Require Export TypedVar.
+Require Export SyntaxSeq.
+Require Export SmallStepSeq.
+Require Export DenotationFacts.
+Require Export DenotationSeq.
+Require Export Eqit.
+Require Export Rutt.
+Require Export RuttFacts.
+Require Import ITree.Basics.HeterogeneousRelations.
+Require Export InterpMTreeFacts.
+Import List.ListNotations.
+Open Scope list_scope.
+From Equations Require Import Equations Signature.
+Require Import Coq.Program.Equality.
+Require Import ExtLib.Structures.Monad.
+Import MonadNotation.
+Local Open Scope monad_scope.
+
+Require Export TypesEquiv.
+
+Definition commute_remove_rel {R MR xR} (rel : Rel (denote_mrec_ctx (denote_mfix_ctx (remove R MR xR) ) ) (denote_mrec_ctx (denote_mfix_ctx (remove R MR xR) ))) :
+  Rel (denote_remainder (denote_mfix_ctx MR) (denote_var xR) ) (denote_remainder (denote_mfix_ctx MR) (denote_var xR) ) :=
+  fun d1 d2 => 
+    rel (projT1 (remove_denote xR d1) ) (projT1 (remove_denote xR d2)).
+
+Definition commute_remove_post_rel {R MR xR} (rel : PostRel (denote_mrec_ctx (denote_mfix_ctx (remove R MR xR) ) ) (denote_mrec_ctx (denote_mfix_ctx (remove R MR xR) ))) :
+  PostRel (denote_remainder (denote_mfix_ctx MR) (denote_var xR) ) (denote_remainder (denote_mfix_ctx MR) (denote_var xR) ) :=
+  fun d1 d2 a b =>
+      let '(d1' && f1) := remove_denote xR d1 in
+      let '(d2' && f2) := remove_denote xR d2 in
+      exists a' b',
+        a = f1 a' ->
+        b = f2 b' ->
+        rel d1' d2' a' b'.
+
+Definition commute_remove_post_rel' {R MR xR} (rel : PostRel (denote_mrec_ctx (denote_mfix_ctx (remove R MR xR) ) ) (denote_mrec_ctx (denote_mfix_ctx (remove R MR xR) ))) :
+  PostRel (denote_remainder (denote_mfix_ctx MR) (denote_var xR) ) (denote_remainder (denote_mfix_ctx MR) (denote_var xR) ) :=
+  fun d1 d2 a b =>
+    forall (H1 : denote_remainder (denote_mfix_ctx MR) (denote_var xR) = (denote_mrec_ctx (denote_mfix_ctx (remove R MR xR) ))) (H2 : encodes d1 = encodes (id_eq H1 d1) ) 
+      (H3 : encodes d2 = encodes (id_eq H1 d2) ), 
+      rel (id_eq H1 d1) (id_eq H1 d2) (id_eq H2 a) (id_eq H3 b)
+.
+
+(* maybe the difficulty I am having now is an indication that I should rewrite the language *)
+
+Transparent denote_var.
+
+(* try to come up with something more general *)
+Lemma commute_remove_post_rel_correct R MR xR : forall
+      (rel : PostRel (denote_mrec_ctx (denote_mfix_ctx (remove R MR xR)))
+         (denote_mrec_ctx (denote_mfix_ctx (remove R MR xR)))) 
+      d1 d2 d1' d2' a b a' b',
+  d1 ~= d1' -> d2 ~= d2' -> a ~= a' -> b ~= b' -> 
+  rel d1' d2' a' b' -> commute_remove_post_rel rel d1 d2 a b.
+Proof.
+  intros. red.
+  destruct (remove_denote xR d1) eqn : Heq1.
+  destruct (remove_denote xR d2) eqn : Heq2.
+  exists a'.
+  dependent induction xR.
+  - intros.
+    red. simpl remove_denote. simpl. exists a0. exists b.
+    intros. subst. auto.
+  - intros. red. simpl remove_denote.
+    destruct d1; destruct d2.
+    + exists a0. exists b0. intros. subst.
+      destruct d1'; destruct d2'.
+      * simpl denote_var in *. cbn in a0.  eapply IHxR in H3; try eapply H1. 4 : { eapply H1. eauto.
+      2 : { injection H.
+      admit.
+    +
+      cbn in a0, b0. cbn in a'. 
+    simpl remove in *. simpl. cbn.
+
+Notation mfix_pre_equiv_insert MR R xR := (InsertPreRel (denote_var xR) (denote_var xR) (call_frame_pre_equiv R) (commute_remove_rel (mfix_pre_equiv (remove R MR xR)) )).
+
+
+(**)
+Lemma mfix_pre_equiv_position (MR : mfix_ctx) (R : call_frame)
+      (t1 t2 : type) (xR : var R MR) (x : var (t1, t2) R) 
+      (v1 v2 : denote_type t1) (d1 d2 : denote_mrec_ctx (denote_mfix_ctx MR)) :
+  d1 = projT1 (call_mrec x xR v1) ->
+  d2 = projT1 (call_mrec x xR v2) ->
+  types_equiv t1 v1 v2 ->
+  mfix_pre_equiv MR d1 d2.
+Proof.
+  revert x. dependent induction xR.
+  - setoid_rewrite call_mrec_equation_1. intros x.
+    dependent induction x.
+    + setoid_rewrite call_mrec_call_frame_equation_1. 
+      intros. cbn in H, H0. subst. constructor. constructor. auto.
+    + destruct b as [t3 t4]. setoid_rewrite call_mrec_call_frame_equation_2.
+      intros. specialize IHx with (x0 := x) (v1 := v1) (v2 := v2); eauto.
+      destruct (call_mrec_call_frame x v1) eqn : Heq1.
+      destruct (call_mrec_call_frame x v2) eqn : Heq2.
+      simpl projT1 in IHx. simpl in H, H0. specialize (IHx (inl x1) (inl x0)). 
+      eapply IHx in H1; eauto.
+      subst. rewrite mfix_pre_equiv_equation_2. constructor.
+      rewrite call_frame_pre_equiv_equation_2. constructor.
+      rewrite mfix_pre_equiv_equation_2 in H1. inversion H1. auto.
+  - setoid_rewrite call_mrec_equation_2. intros.
+    destruct (call_mrec x xR v1) eqn : Heq1.
+    destruct (call_mrec x xR v2) eqn : Heq2.
+    subst. constructor. eapply IHxR; eauto. rewrite Heq1. auto.
+    rewrite Heq2. auto.
+Qed.
+
+Lemma mfix_pre_equiv_position_inv (MR : mfix_ctx) (R : call_frame)
+      (t1 t2 : type) (xR : var R MR) (x : var (t1, t2) R) 
+      (v1 v2 : denote_type t1) (d1 d2 : denote_mrec_ctx (denote_mfix_ctx MR)) :
+  d1 = projT1 (call_mrec x xR v1) ->
+  d2 = projT1 (call_mrec x xR v2) ->
+  mfix_pre_equiv MR d1 d2 ->
+  types_equiv t1 v1 v2.
+Proof.
+  revert x. generalize dependent d1. generalize dependent d2.
+  dependent induction xR.
+  - setoid_rewrite call_mrec_equation_1. intros d2 d1 x.
+    generalize dependent d2. generalize dependent d1.
+    dependent induction x.
+    + setoid_rewrite call_mrec_call_frame_equation_1.
+      simpl projT1. intros. subst.
+      rewrite mfix_pre_equiv_equation_2 in H1.
+      dependent destruction H1.
+      rewrite call_frame_pre_equiv_equation_2 in H.
+      dependent destruction H. auto.
+    + destruct b. setoid_rewrite call_mrec_call_frame_equation_2.
+      intros.
+      specialize (IHx t2 t1 v1 v2 x eq_refl JMeq_refl).
+      destruct (call_mrec_call_frame x v1) eqn : Heq1.
+      destruct (call_mrec_call_frame x v2) eqn : Heq2.
+      cbn in H, H0. simpl projT1 in IHx. subst.
+      rewrite mfix_pre_equiv_equation_2 in H1.
+      dependent destruction H1.
+      rewrite call_frame_pre_equiv_equation_2 in H.
+      dependent destruction H. eapply IHx; eauto.
+      constructor; auto.
+  - setoid_rewrite call_mrec_equation_2.
+    intros.
+    destruct (call_mrec x xR v1) eqn : Heq1.
+    destruct (call_mrec x xR v2) eqn : Heq2.
+    cbn in H, H0. subst.
+    specialize (IHxR v1 v2 x1 x0 x).
+    apply IHxR.
+    rewrite Heq1. auto. rewrite Heq2. auto.
+    rewrite mfix_pre_equiv_equation_2 in H1.
+    dependent destruction H1. auto.
+Qed.
+
+Lemma denote_mfix_exists (MR : mfix_ctx) (d : denote_mrec_ctx (denote_mfix_ctx MR)) : exists (R : call_frame) xR t1 t2 (x : var (t1,t2) R) v,
+    d = projT1 (call_mrec x xR v).
+Proof.
+  revert d. induction MR.
+  - intros. destruct d.
+  - intros. destruct d.
+    + exists a. exists (VarZ). setoid_rewrite call_mrec_equation_1.
+      clear IHMR. revert d. induction a.
+      intros [].
+      intros. simpl in d. destruct a. destruct d.
+      * exists t. exists t0. exists VarZ. 
+        setoid_rewrite call_mrec_call_frame_equation_1. 
+        cbn. eexists. eauto.
+      * specialize (IHa d). 
+        destruct IHa as [ t1 [t2 [x [v Hd] ] ] ].
+        exists t1. exists t2. exists (VarS x). exists v.
+        setoid_rewrite call_mrec_call_frame_equation_2.
+        destruct (call_mrec_call_frame x v).
+        injection Hd. intros. subst. auto.
+    + specialize (IHMR d).
+      destruct IHMR as [R [xR [t1 [t2 [x [v Hd] ] ] ]]].
+      exists R. exists (VarS xR). exists t1. exists t2. exists x. exists v.
+      simp call_mrec. destruct (call_mrec x xR v).
+      subst. auto.
+Qed.
+(* may need to do again for the insert rel version *)
+Lemma mfix_pre_equiv_position_inv_call1 (MR : mfix_ctx) (R1 R2 : call_frame)
+      (t1 t2 t3 t4 : type) (xR : var R1 MR) (yR : var R2 MR) 
+      (x : var (t1, t2) R1) (y : var (t3,t4) R2) 
+      v1 v2 (d1 d2 : denote_mrec_ctx (denote_mfix_ctx MR)) :
+  d1 = projT1 (call_mrec x xR v1) ->
+  d2 = projT1 (call_mrec y yR v2) ->
+  mfix_pre_equiv MR d1 d2 ->
+  R1 = R2.
+Proof.
+  generalize dependent d2. generalize dependent d1.
+  revert x y v1 v2 yR. dependent induction xR.
+  - setoid_rewrite call_mrec_equation_1.
+    intros. destruct (call_mrec_call_frame x v1) as [d1' f1] eqn : Heq1.
+    cbn in H. rewrite H in H1. rewrite mfix_pre_equiv_equation_2 in H1.  
+    dependent destruction H1.
+    dependent destruction yR.
+    2 : { setoid_rewrite call_mrec_equation_2 in H0.
+          destruct (call_mrec y yR v2); discriminate. }
+    setoid_rewrite call_mrec_equation_1 in H0.
+    destruct (call_mrec_call_frame y v2) as [d2' f2] eqn : Heq2.
+    auto.
+  - setoid_rewrite call_mrec_equation_2.
+    intros. destruct (call_mrec x xR v1) as [d1' f1] eqn: Heq1.
+    subst. simpl projT1 in H1.
+    dependent destruction yR.
+    + setoid_rewrite call_mrec_equation_1 in H1.
+      destruct (call_mrec_call_frame y v2). 
+      simpl in H1;
+      dependent destruction H1.
+    + setoid_rewrite call_mrec_equation_2 in H1.
+      destruct (call_mrec y yR v2) as [d2' f2] eqn : Heq2.
+      rewrite mfix_pre_equiv_equation_2 in H1.
+      dependent destruction H1. eapply IHxR; eauto.
+      rewrite Heq1, Heq2. auto.
+Qed.
+
+Lemma mfix_pre_equiv_position_inv_call2 (MR : mfix_ctx) R
+      (t1 t2 t3 t4 : type) (xR : var R MR) (yR : var R MR) 
+      (x : var (t1, t2) R) (y : var (t3,t4) R) 
+      v1 v2 (d1 d2 : denote_mrec_ctx (denote_mfix_ctx MR)) :
+  d1 = projT1 (call_mrec x xR v1) ->
+  d2 = projT1 (call_mrec y yR v2) ->
+  mfix_pre_equiv MR d1 d2 ->
+  t1 = t3 /\ t2 = t4 /\ xR = yR.
+Proof.
+  generalize dependent d2. generalize dependent d1.
+  revert x y v1 v2 yR. dependent induction xR.
+  - setoid_rewrite call_mrec_equation_1.
+    intros. destruct (call_mrec_call_frame x v1) as [d1' f1] eqn : Heq1.
+    cbn in H. rewrite H in H1. rewrite mfix_pre_equiv_equation_2 in H1.  
+    dependent destruction H1.
+    dependent destruction yR.
+    2 : { setoid_rewrite call_mrec_equation_2 in H0.
+          destruct (call_mrec y yR v2); discriminate. }
+    setoid_rewrite call_mrec_equation_1 in H0.
+    destruct (call_mrec_call_frame y v2) as [d2' f2] eqn : Heq2.
+    injection H0. intros. subst a2. clear H0.
+    revert Heq1 Heq2 H1. generalize dependent d2'. generalize dependent d1'.
+    revert v1 v2 y. dependent induction x.
+    + setoid_rewrite call_mrec_call_frame_equation_1. intros.
+      injection Heq1. intros. subst.
+      rewrite call_frame_pre_equiv_equation_2 in H1. 
+      dependent destruction H1.
+      dependent destruction y. auto.
+      simp call_mrec_call_frame in Heq2.
+      destruct (call_mrec_call_frame y v2). discriminate.
+    + destruct b. setoid_rewrite call_mrec_call_frame_equation_2. intros.
+      destruct (call_mrec_call_frame x v1) as [d1'' f1'] eqn : Heq3.
+      injection Heq1. intros. subst.
+      rewrite call_frame_pre_equiv_equation_2 in H1.
+      dependent destruction H1.
+      dependent destruction y.
+      simp call_mrec_call_frame in Heq2. discriminate.
+      simp call_mrec_call_frame in Heq2.
+      destruct (call_mrec_call_frame y v2) as [d2' f2'] eqn : Heq4.
+      injection Heq2. intros. subst b2. eapply IHx in H; eauto. 
+      decompose record H. subst. repeat split; auto.
+  - setoid_rewrite call_mrec_equation_2. intros.
+    destruct (call_mrec x xR v1) as [d1' f1] eqn: Heq1.
+    subst. simpl projT1 in H1.
+    dependent destruction yR.
+    + setoid_rewrite call_mrec_equation_1 in H1.
+      destruct (call_mrec_call_frame y v2). 
+      simpl in H1;
+      dependent destruction H1.
+    + setoid_rewrite call_mrec_equation_2 in H1.
+      destruct (call_mrec y yR v2) as [d2' f2] eqn : Heq2.
+      rewrite mfix_pre_equiv_equation_2 in H1.
+      dependent destruction H1. 
+      eapply IHxR in H; eauto.
+      2 : rewrite Heq1; auto.
+      2  : rewrite Heq2; auto.
+      decompose record H. subst. repeat split; auto.
+Qed.
+
+Lemma mfix_pre_equiv_position_inv_call3 (MR : mfix_ctx) R
+      (t1 t2: type) (xR : var R MR)
+      (x y : var (t1, t2) R)
+      v1 v2 (d1 d2 : denote_mrec_ctx (denote_mfix_ctx MR)) :
+  d1 = projT1 (call_mrec x xR v1) ->
+  d2 = projT1 (call_mrec y xR v2) ->
+  mfix_pre_equiv MR d1 d2 ->
+  x = y.
+Proof.
+  generalize dependent d2. generalize dependent d1.
+  revert x y v1 v2. dependent induction xR.
+  - setoid_rewrite call_mrec_equation_1.
+    intros. destruct (call_mrec_call_frame x v1) as [d1' f1] eqn : Heq1.
+    cbn in H. rewrite H in H1. rewrite mfix_pre_equiv_equation_2 in H1.  
+    dependent destruction H1.
+    destruct (call_mrec_call_frame y v2) as [d2' f2] eqn : Heq2.
+    injection H0. intros. subst a2. clear H0.
+    revert Heq1 Heq2 H1. generalize dependent d2'. generalize dependent d1'.
+    revert v1 v2 y. dependent induction x.
+    + setoid_rewrite call_mrec_call_frame_equation_1. intros.
+      injection Heq1. intros. subst.
+      rewrite call_frame_pre_equiv_equation_2 in H1. 
+      dependent destruction H1.
+      dependent destruction y. auto.
+      simp call_mrec_call_frame in Heq2.
+      destruct (call_mrec_call_frame y v2). discriminate.
+    + destruct b. setoid_rewrite call_mrec_call_frame_equation_2. intros.
+      destruct (call_mrec_call_frame x v1) as [d1'' f1'] eqn : Heq3.
+      injection Heq1. intros. subst.
+      rewrite call_frame_pre_equiv_equation_2 in H1.
+      dependent destruction H1.
+      dependent destruction y.
+      simp call_mrec_call_frame in Heq2. discriminate.
+      simp call_mrec_call_frame in Heq2.
+      destruct (call_mrec_call_frame y v2) as [d2' f2'] eqn : Heq4.
+      injection Heq2. intros. subst b2. 
+      enough (x = y); subst; auto.
+      eapply IHx; eauto.
+  - setoid_rewrite call_mrec_equation_2. intros.
+    destruct (call_mrec x xR v1) as [d1' f1] eqn: Heq1.
+    subst. simpl projT1 in H1.
+    destruct (call_mrec y xR v2) as [d2' f2] eqn : Heq2.
+    rewrite mfix_pre_equiv_equation_2 in H1.
+    dependent destruction H1. eapply IHxR; eauto.
+    rewrite Heq1, Heq2. auto.
+Qed.
+
+
+
+Lemma insert_pre_rel_mfix_pre_equiv_1 (MR : mfix_ctx) (R : call_frame) (xR : var R MR) : 
+  forall x y, 
+    mfix_pre_equiv MR x y ->
+  InsertPreRel (denote_var xR) (denote_var xR) (call_frame_pre_equiv R) (commute_remove_rel (mfix_pre_equiv (remove R MR xR)) ) x y.
+Proof.
+  induction xR.
+  - intros. rewrite mfix_pre_equiv_equation_2 in H.
+    red. dependent destruction H.
+    + constructor. auto.
+    + constructor. red.
+      setoid_rewrite remove_denote_equation_1.
+      Transparent remove. cbn. Opaque remove. auto.
+  - intros. rewrite mfix_pre_equiv_equation_2 in H. dependent destruction H. 
+     { do 2 constructor; auto. }
+     simpl denote_var. red. 
+     eapply IHxR in H. red in H.
+     dependent destruction H.
+     + destruct 
+         ((bring_to_front (denote_mfix_ctx l) (denote_var xR) b1))
+         eqn : Heq1; cbn in x0; subst; try discriminate.
+       unfold denote_mfix_ctx. simpl.
+       rewrite bring_to_front_equation_5.
+       setoid_rewrite Heq1.
+       simpl.
+       destruct 
+         ((bring_to_front (denote_mfix_ctx l) (denote_var xR) b2))
+         eqn : Heq2; cbn in x; subst; try discriminate.
+       unfold denote_mfix_ctx. simpl.
+       rewrite bring_to_front_equation_5.
+       setoid_rewrite Heq2. constructor.
+       auto.
+     + destruct 
+         ((bring_to_front (denote_mfix_ctx l) (denote_var xR) b1))
+         eqn : Heq1; cbn in x0; subst; try discriminate.
+       unfold denote_mfix_ctx. simpl.
+       rewrite bring_to_front_equation_5.
+       setoid_rewrite Heq1.
+       simpl.
+       destruct 
+         ((bring_to_front (denote_mfix_ctx l) (denote_var xR) b2))
+         eqn : Heq2; cbn in x; subst; try discriminate.
+       unfold denote_mfix_ctx. simpl.
+       rewrite bring_to_front_equation_5.
+       setoid_rewrite Heq2.
+       constructor.
+       clear - H. red. Transparent remove_denote.
+       red in H.
+       simpl remove_denote.
+       Transparent remove. simpl remove. simpl.
+       destruct (remove_denote xR b0);
+         destruct (remove_denote xR b3).
+       constructor. auto.
+Qed.
+
+(* now that I've got this proof done, maybe think a bit if it can be improved *)
+
+Lemma insert_pre_rel_mfix_pre_equiv_2 (MR : mfix_ctx) (R : call_frame) (xR : var R MR) : 
+  forall d1 d2, 
+  InsertPreRel (denote_var xR) (denote_var xR) (call_frame_pre_equiv R) (commute_remove_rel (mfix_pre_equiv (remove R MR xR)) ) d1 d2 -> 
+  mfix_pre_equiv MR d1 d2.
+Proof.
+  intros d1 d2 H. red in H.
+  remember (bring_to_front (denote_mfix_ctx MR) (denote_var xR) d1) as d1'.
+  remember (bring_to_front (denote_mfix_ctx MR) (denote_var xR) d2) as d2'.
+  dependent destruction H.
+  - destruct d1' as [ [d1' | d1'] f]; try discriminate.
+    destruct d2' as [ [d2' | d2'] g]; try discriminate.
+    injection x. injection x0. intros. subst. 
+    revert Heqd1' Heqd2' H. clear x x0.
+    generalize dependent d1. generalize dependent d2.
+    revert d1' d2'. dependent induction xR.
+    + simpl denote_var. intros.
+      destruct d1.
+      2 : { setoid_rewrite bring_to_front_equation_3 in Heqd1'. discriminate. }
+      setoid_rewrite bring_to_front_equation_2 in Heqd1'. 
+      injection Heqd1'. intros. subst.
+      destruct d2.
+      2 : { setoid_rewrite bring_to_front_equation_3 in Heqd2'. discriminate. }
+      setoid_rewrite bring_to_front_equation_2 in Heqd2'. 
+      rewrite mfix_pre_equiv_equation_2. constructor.
+      injection Heqd2'. intros. subst. auto.
+    + simpl denote_var. intros.
+      destruct d1.
+      { setoid_rewrite bring_to_front_equation_4 in Heqd1'. discriminate. }
+      destruct d2.
+      { setoid_rewrite bring_to_front_equation_4 in Heqd2'. discriminate. }
+      setoid_rewrite bring_to_front_equation_5 in Heqd1'.
+      destruct (bring_to_front
+                ((fix map (l : list mrec_ctx) : mrec_ctx :=
+                    match l with
+                    | [] => []
+                    | a :: t => denote_mrec_ctx a && encoded_mrec_ctx a :: map t
+                    end)
+                   ((fix map (l : mfix_ctx) : list mrec_ctx :=
+                       match l with
+                       | [] => []
+                       | a :: t =>
+                           List.map
+                             (fun '(t1, t2) =>
+                              denote_type t1 && inout_encoded (denote_type t1) (denote_type t2)) a
+                           :: map t
+                       end) l)) (denote_var xR) d) eqn : Heq1.
+      destruct x; try discriminate. injection Heqd1'. intros. subst.
+      setoid_rewrite bring_to_front_equation_5 in Heqd2'.
+      destruct (bring_to_front
+                ((fix map (l : list mrec_ctx) : mrec_ctx :=
+                    match l with
+                    | [] => []
+                    | a :: t => denote_mrec_ctx a && encoded_mrec_ctx a :: map t
+                    end)
+                   ((fix map (l : mfix_ctx) : list mrec_ctx :=
+                       match l with
+                       | [] => []
+                       | a :: t =>
+                           List.map
+                             (fun '(t1, t2) =>
+                              denote_type t1 && inout_encoded (denote_type t1) (denote_type t2)) a
+                           :: map t
+                       end) l)) (denote_var xR) d0) eqn : Heq2.
+      destruct x; try discriminate. injection Heqd2'. intros. subst.
+      rewrite mfix_pre_equiv_equation_2. constructor.
+      eapply IHxR; eauto.
+  - subst. red in H. generalize dependent xR. intros xR.
+    dependent induction xR.
+    + simpl remove_denote. simpl projT1. intros.
+      destruct ((bring_to_front (denote_mfix_ctx (a :: l)) VarZ d1)) as [d1' f1] eqn : Heq1.
+      destruct ((bring_to_front (denote_mfix_ctx (a :: l)) VarZ d2)) as [d2' f2] eqn : Heq2.
+      Transparent bring_to_front. cbn in x0. cbn in x.
+      destruct d2; destruct d1; try discriminate.
+      injection x. injection x0. intros. subst.
+      rewrite mfix_pre_equiv_equation_2. constructor.
+      assert (l = remove a (a :: l) VarZ). simp remove. auto.
+      simpl in H. auto.
+    + intros. rewrite mfix_pre_equiv_equation_2.
+      destruct d1; destruct d2; simpl in x0; simpl in x; try injection x; try injection x0; intros;
+        subst.
+      * constructor. simpl in H. dependent destruction H. auto.
+      * cbn in x.
+        destruct (bring_to_front
+             (denote_mfix_ctx'
+                (List.map
+                   (List.map
+                      (fun '(t1, t2) =>
+                       denote_type t1 && inout_encoded (denote_type t1) (denote_type t2))) l))
+             (denote_var xR) d0). destruct x1; try discriminate.
+        destruct b2. discriminate. injection x. intros. subst.
+        simpl in H. destruct (remove_denote xR d1). dependent destruction H.
+      * cbn in x0.
+        destruct (bring_to_front
+             (denote_mfix_ctx'
+                (List.map
+                   (List.map
+                      (fun '(t1, t2) =>
+                       denote_type t1 && inout_encoded (denote_type t1) (denote_type t2))) l))
+             (denote_var xR) d). destruct x1; try discriminate.
+        destruct b1. discriminate. injection x0. intros. subst.
+        simpl in H. destruct (remove_denote xR d1). dependent destruction H.
+      * cbn in x. cbn in x0.
+        destruct (bring_to_front
+              (denote_mfix_ctx'
+                 (List.map
+                    (List.map
+                       (fun '(t1, t2) =>
+                        denote_type t1 && inout_encoded (denote_type t1) (denote_type t2))) l))
+              (denote_var xR) d) eqn : Heq1. destruct x1; try discriminate.
+        injection x0. intros. subst.
+        destruct (bring_to_front
+             (denote_mfix_ctx'
+                (List.map
+                   (List.map
+                      (fun '(t1, t2) =>
+                       denote_type t1 && inout_encoded (denote_type t1) (denote_type t2))) l))
+             (denote_var xR) d0) eqn : Heq2. destruct x1; try discriminate.
+        injection x. intros. subst. constructor.
+        eapply IHxR; eauto.
+        2 : { setoid_rewrite Heq1. simpl. reflexivity. }
+        2 : { setoid_rewrite Heq2. simpl. reflexivity. }
+        simpl remove_denote in H.
+        destruct (remove_denote xR d1). destruct (remove_denote xR d2).
+        cbn in H. dependent destruction H; auto.
+Qed.
+(*
+ipr_intro_l
+     : forall (MR1 MR2 : mrec_ctx) (In1 In2 : Type)
+         (Out1 : EncodedType In1) (Out2 : EncodedType In2)
+         (x : var (In1 && Out1) MR1) (y : var (In2 && Out2) MR2)
+         (RPostInv : PostRel In1 In2)
+         (RPost : PostRel (denote_remainder MR1 x)
+                    (denote_remainder MR2 y))
+         (d1 : denote_mrec_ctx MR1) (d2 : denote_mrec_ctx MR2)
+         (a : encodes d1) (b : encodes d2)
+         (d1' : In1 + denote_remainder MR1 x)
+         (d2' : In2 + denote_remainder MR2 y)
+         (f1 : encodes d1' -> encodes d1)
+         (f2 : encodes d2' -> encodes d2) (a' : encodes d1')
+         (b' : encodes d2'),
+       d1' && f1 = bring_to_front MR1 x d1 ->
+       d2' && f2 = bring_to_front MR2 y d2 ->
+       a = f1 a' ->
+       b = f2 b' ->
+       SumPostRel RPostInv RPost d1' d2' a' b' ->
+       InsertPostRel x y RPostInv RPost d1 d2 a b
+
+
+bring_to_front_call_mrec:
+  forall (t1 t2 : vtype) (R : call_frame) (MR : mfix_ctx)
+    (v : denote_type t1) (xt : var (t1, t2) R) 
+    (xR : var R MR),
+  projT1
+    (bring_to_front (denote_mfix_ctx MR) (denote_var xR)
+       (projT1 (call_mrec xt xR v))) =
+  inl (projT1 (call_mrec_call_frame xt v))
+bring_to_front_call_mrec_neq:
+  forall (t1 t2 : vtype) (R1 R2 : call_frame) (MR : mfix_ctx)
+    (v : denote_type t1) (xt : var (t1, t2) R1) 
+    (xR : var R1 MR) (yR : var R2 MR) (Hneq : var_neq xR yR),
+  projT1
+    (bring_to_front (denote_mfix_ctx MR) (denote_var yR)
+       (projT1 (call_mrec xt xR v))) =
+  inr
+    (projT1
+       (remove_denote' yR
+          (projT1
+             (call_mrec xt
+                (remove_var R2 R1 MR yR xR (var_neq_sym xR yR Hneq)) v))))
+
+
+remove_denote_encodes:
+  forall (R : call_frame) (MR : mfix_ctx) (x : var R MR)
+    (d : denote_remainder (denote_mfix_ctx MR) (denote_var x)),
+  encodes d = encodes (projT1 (remove_denote x d))
+d' ~= d ->
+commute_remove_post_rel R d <->
+R d
+
+
+*)
+
+Lemma insert_post_rel_call1 (MR : mfix_ctx) (R : call_frame) (xR : var R MR) :
+  forall d1 d2 a b, 
+  InsertPostRel (denote_var xR) (denote_var xR) (call_frame_post_equiv R) (commute_remove_post_rel (mfix_post_equiv (remove R MR xR)) ) d1 d2 a b -> True.
+Proof.
+  intros. dependent destruction H. dependent destruction H3.
+  - subst. admit.
+  - red in H3.
+Admitted.
+
+Lemma insert_post_rel_mfix_post_equiv_2 (MR : mfix_ctx) (R : call_frame) (xR : var R MR) : 
+  forall d1 d2 a b, 
+  InsertPostRel (denote_var xR) (denote_var xR) (call_frame_post_equiv R) (commute_remove_post_rel (mfix_post_equiv (remove R MR xR)) ) d1 d2 a b -> mfix_post_equiv MR d1 d2 a b.
+Proof.
+(*
+  intros. 
+  specialize (denote_mfix_exists _ d1) as [R1 [yR [t1 [t2 [y [v1 Hd1]]]]]].
+  specialize (denote_mfix_exists _ d2) as [R2 [zR [t3 [t4 [z [v2 Hd2]]]]]].
+  assert (R1 = R2). admit. subst.
+  assert (yR = zR). admit. subst.
+  assert (t1 = t3). admit. subst.
+  assert (t2 = t4). admit. subst.
+  assert (y = z). admit. subst.
+  destruct (var_eq_neq _ _ _ xR zR).
+  - rename v into Heq. apply var_eq_surj in Heq as HR. subst.
+    apply var_eq_eq in Heq. subst xR.
+    dependent destruction H.
+    (* bring_to_front_call_mrec_neq *)
+    specialize (bring_to_front_call_mrec _ _ _ _ v1 z zR) as Hcall1.
+    specialize (bring_to_front_call_mrec _ _ _ _ v2 z zR) as Hcall2.
+    rewrite <- H in Hcall1. rewrite <- H0 in Hcall2. simpl projT1 in Hcall1. simpl projT1 in Hcall2.
+    subst.
+    dependent destruction H3. cbn in f1. cbn in f2. revert H H0 H3.
+    (* maybe should decompose into call_mrec_call_frame for these*)
+    (* assert that both f1 and f2 are the id function*)
+    (* in this case, use Heq to show that H is equiv to a prove of call_frame_post_equiv _ (call_mrec_call_frame z v2) *)
+    admit.
+  - (* these inductions are going to be hideous *) *) Admitted.
+Lemma insert_post_rel_mfix_post_equiv_1 (MR : mfix_ctx) (R : call_frame) (xR : var R MR) : 
+  forall d1 d2 a b, 
+    mfix_post_equiv MR d1 d2 a b ->
+  InsertPostRel (denote_var xR) (denote_var xR) (call_frame_post_equiv R) (commute_remove_post_rel (mfix_post_equiv (remove R MR xR)) ) d1 d2 a b.
+Proof.
+Admitted.
+(*
+  intros d1 d2.
+  specialize (denote_mfix_exists _ d1) as [R1 [yR [t1 [t2 [y [v1 Hd1]]]]]].
+  specialize (denote_mfix_exists _ d2) as [R2 [zR [t3 [t4 [z [v2 Hd2]]]]]].
+  specialize (call_mrec_encodes t1 t2 R1 _ y yR v1) as Hy.
+  rewrite <- Hd1 in Hy.
+  (* maybe I should rewrite Insert in terms of this decomposition, or maybe just a proof that relates it to a similar def *)
+  
+  subst.
+
+  (* I think a creative solution is warranted here *)
+  induction xR.
+  - intros. rewrite mfix_post_equiv_equation_2 in H.
+    simpl denote_var.
+    dependent destruction H.
+    + econstructor.
+    unfold commute_remove_post_rel. 
+    econstructor.
+    simpl remove. cbn.
+    econstructor; eauto.
+    dependent destruction H.
+    + econstructor. auto.
+    + constructor. red.
+      setoid_rewrite remove_denote_equation_1.
+      Transparent remove. cbn. Opaque remove. auto.
+  - intros. rewrite mfix_pre_equiv_equation_2 in H. dependent destruction H. 
+     { do 2 constructor; auto. }
+     simpl denote_var. red. 
+     eapply IHxR in H. red in H.
+     dependent destruction H.
+     + destruct 
+         ((bring_to_front (denote_mfix_ctx l) (denote_var xR) b1))
+         eqn : Heq1; cbn in x0; subst; try discriminate.
+       unfold denote_mfix_ctx. simpl.
+       rewrite bring_to_front_equation_5.
+       setoid_rewrite Heq1.
+       simpl.
+       destruct 
+         ((bring_to_front (denote_mfix_ctx l) (denote_var xR) b2))
+         eqn : Heq2; cbn in x; subst; try discriminate.
+       unfold denote_mfix_ctx. simpl.
+       rewrite bring_to_front_equation_5.
+       setoid_rewrite Heq2. constructor.
+       auto.
+     + destruct 
+         ((bring_to_front (denote_mfix_ctx l) (denote_var xR) b1))
+         eqn : Heq1; cbn in x0; subst; try discriminate.
+       unfold denote_mfix_ctx. simpl.
+       rewrite bring_to_front_equation_5.
+       setoid_rewrite Heq1.
+       simpl.
+       destruct 
+         ((bring_to_front (denote_mfix_ctx l) (denote_var xR) b2))
+         eqn : Heq2; cbn in x; subst; try discriminate.
+       unfold denote_mfix_ctx. simpl.
+       rewrite bring_to_front_equation_5.
+       setoid_rewrite Heq2.
+       constructor.
+       clear - H. red. Transparent remove_denote.
+       red in H.
+       simpl remove_denote.
+       Transparent remove. simpl remove. simpl.
+       destruct (remove_denote xR b0);
+         destruct (remove_denote xR b3).
+       constructor. auto.
+Qed.
+*)
